experiments/coq/Future.v
@@ -1,0 +1,32 @@
+Require Import Coq.Strings.String.
+Require Import Coq.Init.Datatypes.
+Open Scope type_scope.
+
+Definition Exn : Set := string.
+
+Inductive Future (A : Type) : Type :=
+  mkFuture : Exn + A -> Future A.
+
+Arguments mkFuture {_} _.
+
+Definition runFuture {A} (fa : Future A) : Exn + A :=
+  match fa with
+    mkFuture ea => ea
+  end.
+
+Definition retFuture {A} (a : A) : Future A :=
+  mkFuture (inr a).
+
+Definition mapFuture {A B} (fa : Future A) (f : A -> B) : Future B :=
+  match fa with
+  | mkFuture (inl e) => mkFuture (inl e)
+  | mkFuture (inr a) => mkFuture (inr (f a))
+  end.
+
+Definition bindFuture {A B} (fa : Future A) (f : A -> Future B) : Future B :=
+  match fa with
+  | mkFuture (inl e) => mkFuture (inl e)
+  | mkFuture (inr a) => f a
+  end.
+
+Opaque runFuture retFuture mapFuture bindFuture.
